pulse/src/ocaml/plugin/Pulse_Extract_Register.ml
@@ -1,6 +1,6 @@
 let extractor
   : FStar_Extraction_ML_Modul.extension_extractor
-  = fun uenv tm ->
+  = fun uenv sigelt tm ->
       let ps = 
         FStar_Tactics_V2_Basic.proofstate_of_goals
             FStar_Compiler_Range.dummyRange
@@ -8,7 +8,8 @@ let extractor
             [] []
       in
       let result = Pulse_Extract_Main.extract_pulse
-                            uenv 
+                            uenv
+                            sigelt
                             (Pulse_RuntimeUtils.unembed_st_term_for_extraction 
                               (Obj.magic tm))
                             ps in
