pulse/src/ocaml/plugin/generated/Pulse_Extract_Main.ml
@@ -68,12 +68,12 @@ let (extend_env :
         (FStar_Sealed.seal
            (Obj.magic
               (FStar_Range.mk_range "Pulse.Extract.Main.fst"
-                 (Prims.of_int (42)) (Prims.of_int (15)) (Prims.of_int (42))
+                 (Prims.of_int (45)) (Prims.of_int (15)) (Prims.of_int (45))
                  (Prims.of_int (41)))))
         (FStar_Sealed.seal
            (Obj.magic
               (FStar_Range.mk_range "Pulse.Extract.Main.fst"
-                 (Prims.of_int (42)) (Prims.of_int (44)) (Prims.of_int (50))
+                 (Prims.of_int (45)) (Prims.of_int (44)) (Prims.of_int (53))
                  (Prims.of_int (64)))))
         (Obj.magic (term_as_mlty g b.Pulse_Syntax_Base.binder_ty))
         (fun uu___ ->
@@ -83,13 +83,13 @@ let (extend_env :
                    (FStar_Sealed.seal
                       (Obj.magic
                          (FStar_Range.mk_range "Pulse.Extract.Main.fst"
-                            (Prims.of_int (43)) (Prims.of_int (12))
-                            (Prims.of_int (43)) (Prims.of_int (29)))))
+                            (Prims.of_int (46)) (Prims.of_int (12))
+                            (Prims.of_int (46)) (Prims.of_int (29)))))
                    (FStar_Sealed.seal
                       (Obj.magic
                          (FStar_Range.mk_range "Pulse.Extract.Main.fst"
-                            (Prims.of_int (43)) (Prims.of_int (32))
-                            (Prims.of_int (50)) (Prims.of_int (64)))))
+                            (Prims.of_int (46)) (Prims.of_int (32))
+                            (Prims.of_int (53)) (Prims.of_int (64)))))
                    (FStar_Tactics_Effect.lift_div_tac
                       (fun uu___ -> Pulse_Typing_Env.fresh g.coreenv))
                    (fun uu___ ->
@@ -100,16 +100,16 @@ let (extend_env :
                                  (Obj.magic
                                     (FStar_Range.mk_range
                                        "Pulse.Extract.Main.fst"
-                                       (Prims.of_int (44))
+                                       (Prims.of_int (47))
                                        (Prims.of_int (18))
-                                       (Prims.of_int (44))
+                                       (Prims.of_int (47))
                                        (Prims.of_int (72)))))
                               (FStar_Sealed.seal
                                  (Obj.magic
                                     (FStar_Range.mk_range
                                        "Pulse.Extract.Main.fst"
-                                       (Prims.of_int (45)) (Prims.of_int (4))
-                                       (Prims.of_int (50))
+                                       (Prims.of_int (48)) (Prims.of_int (4))
+                                       (Prims.of_int (53))
                                        (Prims.of_int (64)))))
                               (FStar_Tactics_Effect.lift_div_tac
                                  (fun uu___ ->
@@ -124,17 +124,17 @@ let (extend_env :
                                             (Obj.magic
                                                (FStar_Range.mk_range
                                                   "Pulse.Extract.Main.fst"
-                                                  (Prims.of_int (45))
+                                                  (Prims.of_int (48))
                                                   (Prims.of_int (4))
-                                                  (Prims.of_int (47))
+                                                  (Prims.of_int (50))
                                                   (Prims.of_int (67)))))
                                          (FStar_Sealed.seal
                                             (Obj.magic
                                                (FStar_Range.mk_range
                                                   "Pulse.Extract.Main.fst"
-                                                  (Prims.of_int (47))
-                                                  (Prims.of_int (68))
                                                   (Prims.of_int (50))
+                                                  (Prims.of_int (68))
+                                                  (Prims.of_int (53))
                                                   (Prims.of_int (64)))))
                                          (Obj.magic
                                             (FStar_Tactics_Effect.tac_bind
@@ -142,17 +142,17 @@ let (extend_env :
                                                   (Obj.magic
                                                      (FStar_Range.mk_range
                                                         "Pulse.Extract.Main.fst"
-                                                        (Prims.of_int (45))
+                                                        (Prims.of_int (48))
                                                         (Prims.of_int (11))
-                                                        (Prims.of_int (47))
+                                                        (Prims.of_int (50))
                                                         (Prims.of_int (67)))))
                                                (FStar_Sealed.seal
                                                   (Obj.magic
                                                      (FStar_Range.mk_range
                                                         "Pulse.Extract.Main.fst"
-                                                        (Prims.of_int (45))
+                                                        (Prims.of_int (48))
                                                         (Prims.of_int (4))
-                                                        (Prims.of_int (47))
+                                                        (Prims.of_int (50))
                                                         (Prims.of_int (67)))))
                                                (Obj.magic
                                                   (FStar_Tactics_Effect.tac_bind
@@ -160,17 +160,17 @@ let (extend_env :
                                                         (Obj.magic
                                                            (FStar_Range.mk_range
                                                               "Pulse.Extract.Main.fst"
-                                                              (Prims.of_int (47))
+                                                              (Prims.of_int (50))
                                                               (Prims.of_int (38))
-                                                              (Prims.of_int (47))
+                                                              (Prims.of_int (50))
                                                               (Prims.of_int (66)))))
                                                      (FStar_Sealed.seal
                                                         (Obj.magic
                                                            (FStar_Range.mk_range
                                                               "Pulse.Extract.Main.fst"
-                                                              (Prims.of_int (45))
+                                                              (Prims.of_int (48))
                                                               (Prims.of_int (11))
-                                                              (Prims.of_int (47))
+                                                              (Prims.of_int (50))
                                                               (Prims.of_int (67)))))
                                                      (Obj.magic
                                                         (Pulse_Syntax_Printer.term_to_string
@@ -183,17 +183,17 @@ let (extend_env :
                                                                    (Obj.magic
                                                                     (FStar_Range.mk_range
                                                                     "Pulse.Extract.Main.fst"
-                                                                    (Prims.of_int (45))
+                                                                    (Prims.of_int (48))
                                                                     (Prims.of_int (11))
-                                                                    (Prims.of_int (47))
+                                                                    (Prims.of_int (50))
                                                                     (Prims.of_int (67)))))
                                                                 (FStar_Sealed.seal
                                                                    (Obj.magic
                                                                     (FStar_Range.mk_range
                                                                     "Pulse.Extract.Main.fst"
-                                                                    (Prims.of_int (45))
+                                                                    (Prims.of_int (48))
                                                                     (Prims.of_int (11))
-                                                                    (Prims.of_int (47))
+                                                                    (Prims.of_int (50))
                                                                     (Prims.of_int (67)))))
                                                                 (Obj.magic
                                                                    (FStar_Tactics_Effect.tac_bind
@@ -201,9 +201,9 @@ let (extend_env :
                                                                     (Obj.magic
                                                                     (FStar_Range.mk_range
                                                                     "Pulse.Extract.Main.fst"
-                                                                    (Prims.of_int (46))
+                                                                    (Prims.of_int (49))
                                                                     (Prims.of_int (38))
-                                                                    (Prims.of_int (46))
+                                                                    (Prims.of_int (49))
                                                                     (Prims.of_int (58)))))
                                                                     (FStar_Sealed.seal
                                                                     (Obj.magic
@@ -279,13 +279,13 @@ let rec (name_as_mlpath :
                    (FStar_Sealed.seal
                       (Obj.magic
                          (FStar_Range.mk_range "Pulse.Extract.Main.fst"
-                            (Prims.of_int (58)) (Prims.of_int (18))
-                            (Prims.of_int (58)) (Prims.of_int (35)))))
+                            (Prims.of_int (61)) (Prims.of_int (18))
+                            (Prims.of_int (61)) (Prims.of_int (35)))))
                    (FStar_Sealed.seal
                       (Obj.magic
                          (FStar_Range.mk_range "Pulse.Extract.Main.fst"
-                            (Prims.of_int (57)) (Prims.of_int (16))
-                            (Prims.of_int (59)) (Prims.of_int (16)))))
+                            (Prims.of_int (60)) (Prims.of_int (16))
+                            (Prims.of_int (62)) (Prims.of_int (16)))))
                    (Obj.magic (name_as_mlpath xs))
                    (fun uu___ ->
                       FStar_Tactics_Effect.lift_div_tac
@@ -304,12 +304,12 @@ let (extract_constant :
         (FStar_Sealed.seal
            (Obj.magic
               (FStar_Range.mk_range "Pulse.Extract.Main.fst"
-                 (Prims.of_int (64)) (Prims.of_int (12)) (Prims.of_int (64))
+                 (Prims.of_int (67)) (Prims.of_int (12)) (Prims.of_int (67))
                  (Prims.of_int (36)))))
         (FStar_Sealed.seal
            (Obj.magic
               (FStar_Range.mk_range "Pulse.Extract.Main.fst"
-                 (Prims.of_int (64)) (Prims.of_int (39)) (Prims.of_int (68))
+                 (Prims.of_int (67)) (Prims.of_int (39)) (Prims.of_int (71))
                  (Prims.of_int (17)))))
         (FStar_Tactics_Effect.lift_div_tac
            (fun uu___ ->
@@ -322,13 +322,13 @@ let (extract_constant :
                    (FStar_Sealed.seal
                       (Obj.magic
                          (FStar_Range.mk_range "Pulse.Extract.Main.fst"
-                            (Prims.of_int (65)) (Prims.of_int (20))
-                            (Prims.of_int (65)) (Prims.of_int (64)))))
+                            (Prims.of_int (68)) (Prims.of_int (20))
+                            (Prims.of_int (68)) (Prims.of_int (64)))))
                    (FStar_Sealed.seal
                       (Obj.magic
                          (FStar_Range.mk_range "Pulse.Extract.Main.fst"
-                            (Prims.of_int (64)) (Prims.of_int (39))
-                            (Prims.of_int (68)) (Prims.of_int (17)))))
+                            (Prims.of_int (67)) (Prims.of_int (39))
+                            (Prims.of_int (71)) (Prims.of_int (17)))))
                    (FStar_Tactics_Effect.lift_div_tac
                       (fun uu___ ->
                          Pulse_Extract_CompilerLib.term_as_mlexpr
@@ -343,17 +343,17 @@ let (extract_constant :
                                      (Obj.magic
                                         (FStar_Range.mk_range
                                            "Pulse.Extract.Main.fst"
-                                           (Prims.of_int (66))
+                                           (Prims.of_int (69))
                                            (Prims.of_int (10))
-                                           (Prims.of_int (66))
+                                           (Prims.of_int (69))
                                            (Prims.of_int (34)))))
                                   (FStar_Sealed.seal
                                      (Obj.magic
                                         (FStar_Range.mk_range
                                            "Pulse.Extract.Main.fst"
-                                           (Prims.of_int (66))
+                                           (Prims.of_int (69))
                                            (Prims.of_int (4))
-                                           (Prims.of_int (68))
+                                           (Prims.of_int (71))
                                            (Prims.of_int (17)))))
                                   (FStar_Tactics_Effect.lift_div_tac
                                      (fun uu___3 ->
@@ -418,13 +418,13 @@ let rec (extend_env_pat_core :
                        (FStar_Sealed.seal
                           (Obj.magic
                              (FStar_Range.mk_range "Pulse.Extract.Main.fst"
-                                (Prims.of_int (85)) (Prims.of_int (8))
-                                (Prims.of_int (90)) (Prims.of_int (14)))))
+                                (Prims.of_int (88)) (Prims.of_int (8))
+                                (Prims.of_int (93)) (Prims.of_int (14)))))
                        (FStar_Sealed.seal
                           (Obj.magic
                              (FStar_Range.mk_range "Pulse.Extract.Main.fst"
-                                (Prims.of_int (83)) (Prims.of_int (24))
-                                (Prims.of_int (92)) (Prims.of_int (68)))))
+                                (Prims.of_int (86)) (Prims.of_int (24))
+                                (Prims.of_int (95)) (Prims.of_int (68)))))
                        (Obj.magic
                           (FStar_Tactics_Util.fold_left
                              (fun uu___ ->
@@ -436,17 +436,17 @@ let rec (extend_env_pat_core :
                                            (Obj.magic
                                               (FStar_Range.mk_range
                                                  "Pulse.Extract.Main.fst"
-                                                 (Prims.of_int (87))
+                                                 (Prims.of_int (90))
                                                  (Prims.of_int (38))
-                                                 (Prims.of_int (87))
+                                                 (Prims.of_int (90))
                                                  (Prims.of_int (61)))))
                                         (FStar_Sealed.seal
                                            (Obj.magic
                                               (FStar_Range.mk_range
                                                  "Pulse.Extract.Main.fst"
-                                                 (Prims.of_int (86))
+                                                 (Prims.of_int (89))
                                                  (Prims.of_int (44))
-                                                 (Prims.of_int (88))
+                                                 (Prims.of_int (91))
                                                  (Prims.of_int (47)))))
                                         (Obj.magic
                                            (extend_env_pat_core g1 p1))
@@ -471,17 +471,17 @@ let rec (extend_env_pat_core :
                                          (Obj.magic
                                             (FStar_Range.mk_range
                                                "Pulse.Extract.Main.fst"
-                                               (Prims.of_int (92))
+                                               (Prims.of_int (95))
                                                (Prims.of_int (9))
-                                               (Prims.of_int (92))
+                                               (Prims.of_int (95))
                                                (Prims.of_int (58)))))
                                       (FStar_Sealed.seal
                                          (Obj.magic
                                             (FStar_Range.mk_range
                                                "Pulse.Extract.Main.fst"
-                                               (Prims.of_int (92))
+                                               (Prims.of_int (95))
                                                (Prims.of_int (6))
-                                               (Prims.of_int (92))
+                                               (Prims.of_int (95))
                                                (Prims.of_int (68)))))
                                       (Obj.magic
                                          (FStar_Tactics_Effect.tac_bind
@@ -489,17 +489,17 @@ let rec (extend_env_pat_core :
                                                (Obj.magic
                                                   (FStar_Range.mk_range
                                                      "Pulse.Extract.Main.fst"
-                                                     (Prims.of_int (92))
+                                                     (Prims.of_int (95))
                                                      (Prims.of_int (10))
-                                                     (Prims.of_int (92))
+                                                     (Prims.of_int (95))
                                                      (Prims.of_int (57)))))
                                             (FStar_Sealed.seal
                                                (Obj.magic
                                                   (FStar_Range.mk_range
                                                      "Pulse.Extract.Main.fst"
-                                                     (Prims.of_int (92))
+                                                     (Prims.of_int (95))
                                                      (Prims.of_int (9))
-                                                     (Prims.of_int (92))
+                                                     (Prims.of_int (95))
                                                      (Prims.of_int (58)))))
                                             (Obj.magic
                                                (FStar_Tactics_Effect.tac_bind
@@ -507,17 +507,17 @@ let rec (extend_env_pat_core :
                                                      (Obj.magic
                                                         (FStar_Range.mk_range
                                                            "Pulse.Extract.Main.fst"
-                                                           (Prims.of_int (92))
+                                                           (Prims.of_int (95))
                                                            (Prims.of_int (26))
-                                                           (Prims.of_int (92))
+                                                           (Prims.of_int (95))
                                                            (Prims.of_int (52)))))
                                                   (FStar_Sealed.seal
                                                      (Obj.magic
                                                         (FStar_Range.mk_range
                                                            "Pulse.Extract.Main.fst"
-                                                           (Prims.of_int (92))
+                                                           (Prims.of_int (95))
                                                            (Prims.of_int (10))
-                                                           (Prims.of_int (92))
+                                                           (Prims.of_int (95))
                                                            (Prims.of_int (57)))))
                                                   (Obj.magic
                                                      (name_as_mlpath
@@ -542,13 +542,13 @@ let rec (extend_env_pat_core :
                        (FStar_Sealed.seal
                           (Obj.magic
                              (FStar_Range.mk_range "Pulse.Extract.Main.fst"
-                                (Prims.of_int (94)) (Prims.of_int (14))
-                                (Prims.of_int (94)) (Prims.of_int (34)))))
+                                (Prims.of_int (97)) (Prims.of_int (14))
+                                (Prims.of_int (97)) (Prims.of_int (34)))))
                        (FStar_Sealed.seal
                           (Obj.magic
                              (FStar_Range.mk_range "Pulse.Extract.Main.fst"
-                                (Prims.of_int (95)) (Prims.of_int (6))
-                                (Prims.of_int (95)) (Prims.of_int (26)))))
+                                (Prims.of_int (98)) (Prims.of_int (6))
+                                (Prims.of_int (98)) (Prims.of_int (26)))))
                        (Obj.magic (extract_constant g c))
                        (fun c1 ->
                           FStar_Tactics_Effect.lift_div_tac
@@ -568,12 +568,12 @@ let (extend_env_pat :
         (FStar_Sealed.seal
            (Obj.magic
               (FStar_Range.mk_range "Pulse.Extract.Main.fst"
-                 (Prims.of_int (97)) (Prims.of_int (20)) (Prims.of_int (97))
-                 (Prims.of_int (43)))))
+                 (Prims.of_int (100)) (Prims.of_int (20))
+                 (Prims.of_int (100)) (Prims.of_int (43)))))
         (FStar_Sealed.seal
            (Obj.magic
               (FStar_Range.mk_range "Pulse.Extract.Main.fst"
-                 (Prims.of_int (96)) (Prims.of_int (24)) (Prims.of_int (100))
+                 (Prims.of_int (99)) (Prims.of_int (24)) (Prims.of_int (103))
                  (Prims.of_int (72))))) (Obj.magic (extend_env_pat_core g p))
         (fun uu___ ->
            match uu___ with
@@ -597,12 +597,12 @@ let (is_erasable :
       (FStar_Sealed.seal
          (Obj.magic
             (FStar_Range.mk_range "Pulse.Extract.Main.fst"
-               (Prims.of_int (104)) (Prims.of_int (12)) (Prims.of_int (104))
+               (Prims.of_int (107)) (Prims.of_int (12)) (Prims.of_int (107))
                (Prims.of_int (33)))))
       (FStar_Sealed.seal
          (Obj.magic
             (FStar_Range.mk_range "Pulse.Extract.Main.fst"
-               (Prims.of_int (105)) (Prims.of_int (2)) (Prims.of_int (107))
+               (Prims.of_int (108)) (Prims.of_int (2)) (Prims.of_int (110))
                (Prims.of_int (14)))))
       (Obj.magic (FStar_Tactics_Unseal.unseal p.Pulse_Syntax_Base.effect_tag))
       (fun tag ->
@@ -723,12 +723,12 @@ let rec (extract :
         (FStar_Sealed.seal
            (Obj.magic
               (FStar_Range.mk_range "Pulse.Extract.Main.fst"
-                 (Prims.of_int (174)) (Prims.of_int (24))
-                 (Prims.of_int (174)) (Prims.of_int (48)))))
+                 (Prims.of_int (177)) (Prims.of_int (24))
+                 (Prims.of_int (177)) (Prims.of_int (48)))))
         (FStar_Sealed.seal
            (Obj.magic
               (FStar_Range.mk_range "Pulse.Extract.Main.fst"
-                 (Prims.of_int (175)) (Prims.of_int (4)) (Prims.of_int (283))
+                 (Prims.of_int (178)) (Prims.of_int (4)) (Prims.of_int (286))
                  (Prims.of_int (7)))))
         (FStar_Tactics_Effect.lift_div_tac
            (fun uu___ ->
@@ -741,42 +741,42 @@ let rec (extract :
                    (FStar_Sealed.seal
                       (Obj.magic
                          (FStar_Range.mk_range "Pulse.Extract.Main.fst"
-                            (Prims.of_int (175)) (Prims.of_int (4))
-                            (Prims.of_int (177)) (Prims.of_int (36)))))
+                            (Prims.of_int (178)) (Prims.of_int (4))
+                            (Prims.of_int (180)) (Prims.of_int (36)))))
                    (FStar_Sealed.seal
                       (Obj.magic
                          (FStar_Range.mk_range "Pulse.Extract.Main.fst"
-                            (Prims.of_int (178)) (Prims.of_int (4))
-                            (Prims.of_int (283)) (Prims.of_int (7)))))
+                            (Prims.of_int (181)) (Prims.of_int (4))
+                            (Prims.of_int (286)) (Prims.of_int (7)))))
                    (Obj.magic
                       (FStar_Tactics_Effect.tac_bind
                          (FStar_Sealed.seal
                             (Obj.magic
                                (FStar_Range.mk_range "Pulse.Extract.Main.fst"
-                                  (Prims.of_int (175)) (Prims.of_int (11))
-                                  (Prims.of_int (177)) (Prims.of_int (36)))))
+                                  (Prims.of_int (178)) (Prims.of_int (11))
+                                  (Prims.of_int (180)) (Prims.of_int (36)))))
                          (FStar_Sealed.seal
                             (Obj.magic
                                (FStar_Range.mk_range "Pulse.Extract.Main.fst"
-                                  (Prims.of_int (175)) (Prims.of_int (4))
-                                  (Prims.of_int (177)) (Prims.of_int (36)))))
+                                  (Prims.of_int (178)) (Prims.of_int (4))
+                                  (Prims.of_int (180)) (Prims.of_int (36)))))
                          (Obj.magic
                             (FStar_Tactics_Effect.tac_bind
                                (FStar_Sealed.seal
                                   (Obj.magic
                                      (FStar_Range.mk_range
                                         "Pulse.Extract.Main.fst"
-                                        (Prims.of_int (177))
+                                        (Prims.of_int (180))
                                         (Prims.of_int (14))
-                                        (Prims.of_int (177))
+                                        (Prims.of_int (180))
                                         (Prims.of_int (35)))))
                                (FStar_Sealed.seal
                                   (Obj.magic
                                      (FStar_Range.mk_range
                                         "Pulse.Extract.Main.fst"
-                                        (Prims.of_int (175))
+                                        (Prims.of_int (178))
                                         (Prims.of_int (11))
-                                        (Prims.of_int (177))
+                                        (Prims.of_int (180))
                                         (Prims.of_int (36)))))
                                (Obj.magic
                                   (Pulse_Syntax_Printer.st_term_to_string p))
@@ -788,17 +788,17 @@ let rec (extract :
                                              (Obj.magic
                                                 (FStar_Range.mk_range
                                                    "Pulse.Extract.Main.fst"
-                                                   (Prims.of_int (175))
+                                                   (Prims.of_int (178))
                                                    (Prims.of_int (11))
-                                                   (Prims.of_int (177))
+                                                   (Prims.of_int (180))
                                                    (Prims.of_int (36)))))
                                           (FStar_Sealed.seal
                                              (Obj.magic
                                                 (FStar_Range.mk_range
                                                    "Pulse.Extract.Main.fst"
-                                                   (Prims.of_int (175))
+                                                   (Prims.of_int (178))
                                                    (Prims.of_int (11))
-                                                   (Prims.of_int (177))
+                                                   (Prims.of_int (180))
                                                    (Prims.of_int (36)))))
                                           (Obj.magic
                                              (FStar_Tactics_Effect.tac_bind
@@ -806,9 +806,9 @@ let rec (extract :
                                                    (Obj.magic
                                                       (FStar_Range.mk_range
                                                          "Pulse.Extract.Main.fst"
-                                                         (Prims.of_int (176))
+                                                         (Prims.of_int (179))
                                                          (Prims.of_int (14))
-                                                         (Prims.of_int (176))
+                                                         (Prims.of_int (179))
                                                          (Prims.of_int (41)))))
                                                 (FStar_Sealed.seal
                                                    (Obj.magic
@@ -850,17 +850,17 @@ let rec (extract :
                                  (Obj.magic
                                     (FStar_Range.mk_range
                                        "Pulse.Extract.Main.fst"
-                                       (Prims.of_int (178))
+                                       (Prims.of_int (181))
                                        (Prims.of_int (7))
-                                       (Prims.of_int (178))
+                                       (Prims.of_int (181))
                                        (Prims.of_int (20)))))
                               (FStar_Sealed.seal
                                  (Obj.magic
                                     (FStar_Range.mk_range
                                        "Pulse.Extract.Main.fst"
-                                       (Prims.of_int (178))
+                                       (Prims.of_int (181))
                                        (Prims.of_int (4))
-                                       (Prims.of_int (283))
+                                       (Prims.of_int (286))
                                        (Prims.of_int (7)))))
                               (Obj.magic (is_erasable p))
                               (fun uu___1 ->
@@ -914,17 +914,17 @@ let rec (extract :
                                                         (Obj.magic
                                                            (FStar_Range.mk_range
                                                               "Pulse.Extract.Main.fst"
-                                                              (Prims.of_int (189))
+                                                              (Prims.of_int (192))
                                                               (Prims.of_int (37))
-                                                              (Prims.of_int (189))
+                                                              (Prims.of_int (192))
                                                               (Prims.of_int (51)))))
                                                      (FStar_Sealed.seal
                                                         (Obj.magic
                                                            (FStar_Range.mk_range
                                                               "Pulse.Extract.Main.fst"
-                                                              (Prims.of_int (188))
+                                                              (Prims.of_int (191))
                                                               (Prims.of_int (32))
-                                                              (Prims.of_int (193))
+                                                              (Prims.of_int (196))
                                                               (Prims.of_int (23)))))
                                                      (Obj.magic
                                                         (extend_env g b))
@@ -940,18 +940,18 @@ let rec (extract :
                                                                     (Obj.magic
                                                                     (FStar_Range.mk_range
                                                                     "Pulse.Extract.Main.fst"
-                                                                    (Prims.of_int (190))
+                                                                    (Prims.of_int (193))
                                                                     (Prims.of_int (19))
-                                                                    (Prims.of_int (190))
+                                                                    (Prims.of_int (193))
                                                                     (Prims.of_int (47)))))
                                                                     (
                                                                     FStar_Sealed.seal
                                                                     (Obj.magic
                                                                     (FStar_Range.mk_range
                                                                     "Pulse.Extract.Main.fst"
-                                                                    (Prims.of_int (190))
-                                                                    (Prims.of_int (50))
                                                                     (Prims.of_int (193))
+                                                                    (Prims.of_int (50))
+                                                                    (Prims.of_int (196))
                                                                     (Prims.of_int (23)))))
                                                                     (
                                                                     FStar_Tactics_Effect.lift_div_tac
@@ -971,17 +971,17 @@ let rec (extract :
                                                                     (Obj.magic
                                                                     (FStar_Range.mk_range
                                                                     "Pulse.Extract.Main.fst"
-                                                                    (Prims.of_int (191))
+                                                                    (Prims.of_int (194))
                                                                     (Prims.of_int (22))
-                                                                    (Prims.of_int (191))
+                                                                    (Prims.of_int (194))
                                                                     (Prims.of_int (36)))))
                                                                     (FStar_Sealed.seal
                                                                     (Obj.magic
                                                                     (FStar_Range.mk_range
                                                                     "Pulse.Extract.Main.fst"
-                                                                    (Prims.of_int (190))
-                                                                    (Prims.of_int (50))
                                                                     (Prims.of_int (193))
+                                                                    (Prims.of_int (50))
+                                                                    (Prims.of_int (196))
                                                                     (Prims.of_int (23)))))
                                                                     (Obj.magic
                                                                     (extract
@@ -1020,17 +1020,17 @@ let rec (extract :
                                                         (Obj.magic
                                                            (FStar_Range.mk_range
                                                               "Pulse.Extract.Main.fst"
-                                                              (Prims.of_int (196))
+                                                              (Prims.of_int (199))
                                                               (Prims.of_int (8))
-                                                              (Prims.of_int (196))
+                                                              (Prims.of_int (199))
                                                               (Prims.of_int (29)))))
                                                      (FStar_Sealed.seal
                                                         (Obj.magic
                                                            (FStar_Range.mk_range
                                                               "Pulse.Extract.Main.fst"
-                                                              (Prims.of_int (196))
+                                                              (Prims.of_int (199))
                                                               (Prims.of_int (8))
-                                                              (Prims.of_int (197))
+                                                              (Prims.of_int (200))
                                                               (Prims.of_int (18)))))
                                                      (Obj.magic
                                                         (term_as_mlexpr g
@@ -1059,17 +1059,17 @@ let rec (extract :
                                                             (Obj.magic
                                                                (FStar_Range.mk_range
                                                                   "Pulse.Extract.Main.fst"
-                                                                  (Prims.of_int (202))
+                                                                  (Prims.of_int (205))
                                                                   (Prims.of_int (21))
-                                                                  (Prims.of_int (202))
+                                                                  (Prims.of_int (205))
                                                                   (Prims.of_int (42)))))
                                                          (FStar_Sealed.seal
                                                             (Obj.magic
                                                                (FStar_Range.mk_range
                                                                   "Pulse.Extract.Main.fst"
-                                                                  (Prims.of_int (202))
+                                                                  (Prims.of_int (205))
                                                                   (Prims.of_int (45))
-                                                                  (Prims.of_int (204))
+                                                                  (Prims.of_int (207))
                                                                   (Prims.of_int (42)))))
                                                          (Obj.magic
                                                             (term_as_mlexpr g
@@ -1083,18 +1083,18 @@ let rec (extract :
                                                                     (Obj.magic
                                                                     (FStar_Range.mk_range
                                                                     "Pulse.Extract.Main.fst"
-                                                                    (Prims.of_int (203))
+                                                                    (Prims.of_int (206))
                                                                     (Prims.of_int (20))
-                                                                    (Prims.of_int (203))
+                                                                    (Prims.of_int (206))
                                                                     (Prims.of_int (40)))))
                                                                     (
                                                                     FStar_Sealed.seal
                                                                     (Obj.magic
                                                                     (FStar_Range.mk_range
                                                                     "Pulse.Extract.Main.fst"
-                                                                    (Prims.of_int (204))
+                                                                    (Prims.of_int (207))
                                                                     (Prims.of_int (10))
-                                                                    (Prims.of_int (204))
+                                                                    (Prims.of_int (207))
                                                                     (Prims.of_int (42)))))
                                                                     (
                                                                     Obj.magic
@@ -1128,17 +1128,17 @@ let rec (extract :
                                                         (Obj.magic
                                                            (FStar_Range.mk_range
                                                               "Pulse.Extract.Main.fst"
-                                                              (Prims.of_int (209))
+                                                              (Prims.of_int (212))
                                                               (Prims.of_int (11))
-                                                              (Prims.of_int (209))
+                                                              (Prims.of_int (212))
                                                               (Prims.of_int (27)))))
                                                      (FStar_Sealed.seal
                                                         (Obj.magic
                                                            (FStar_Range.mk_range
                                                               "Pulse.Extract.Main.fst"
-                                                              (Prims.of_int (209))
+                                                              (Prims.of_int (212))
                                                               (Prims.of_int (8))
-                                                              (Prims.of_int (225))
+                                                              (Prims.of_int (228))
                                                               (Prims.of_int (9)))))
                                                      (Obj.magic
                                                         (is_erasable head))
@@ -1152,17 +1152,17 @@ let rec (extract :
                                                                     (Obj.magic
                                                                     (FStar_Range.mk_range
                                                                     "Pulse.Extract.Main.fst"
-                                                                    (Prims.of_int (211))
+                                                                    (Prims.of_int (214))
                                                                     (Prims.of_int (21))
-                                                                    (Prims.of_int (211))
+                                                                    (Prims.of_int (214))
                                                                     (Prims.of_int (61)))))
                                                                   (FStar_Sealed.seal
                                                                     (Obj.magic
                                                                     (FStar_Range.mk_range
                                                                     "Pulse.Extract.Main.fst"
-                                                                    (Prims.of_int (212))
-                                                                    (Prims.of_int (10))
                                                                     (Prims.of_int (215))
+                                                                    (Prims.of_int (10))
+                                                                    (Prims.of_int (218))
                                                                     (Prims.of_int (24)))))
                                                                   (FStar_Tactics_Effect.lift_div_tac
                                                                     (fun
@@ -1183,17 +1183,17 @@ let rec (extract :
                                                                     (Obj.magic
                                                                     (FStar_Range.mk_range
                                                                     "Pulse.Extract.Main.fst"
-                                                                    (Prims.of_int (212))
+                                                                    (Prims.of_int (215))
                                                                     (Prims.of_int (10))
-                                                                    (Prims.of_int (214))
+                                                                    (Prims.of_int (217))
                                                                     (Prims.of_int (47)))))
                                                                     (FStar_Sealed.seal
                                                                     (Obj.magic
                                                                     (FStar_Range.mk_range
                                                                     "Pulse.Extract.Main.fst"
-                                                                    (Prims.of_int (215))
+                                                                    (Prims.of_int (218))
                                                                     (Prims.of_int (10))
-                                                                    (Prims.of_int (215))
+                                                                    (Prims.of_int (218))
                                                                     (Prims.of_int (24)))))
                                                                     (Obj.magic
                                                                     (FStar_Tactics_Effect.tac_bind
@@ -1201,17 +1201,17 @@ let rec (extract :
                                                                     (Obj.magic
                                                                     (FStar_Range.mk_range
                                                                     "Pulse.Extract.Main.fst"
-                                                                    (Prims.of_int (212))
+                                                                    (Prims.of_int (215))
                                                                     (Prims.of_int (17))
-                                                                    (Prims.of_int (214))
+                                                                    (Prims.of_int (217))
                                                                     (Prims.of_int (47)))))
                                                                     (FStar_Sealed.seal
                                                                     (Obj.magic
                                                                     (FStar_Range.mk_range
                                                                     "Pulse.Extract.Main.fst"
-                                                                    (Prims.of_int (212))
+                                                                    (Prims.of_int (215))
                                                                     (Prims.of_int (10))
-                                                                    (Prims.of_int (214))
+                                                                    (Prims.of_int (217))
                                                                     (Prims.of_int (47)))))
                                                                     (Obj.magic
                                                                     (FStar_Tactics_Effect.tac_bind
@@ -1219,17 +1219,17 @@ let rec (extract :
                                                                     (Obj.magic
                                                                     (FStar_Range.mk_range
                                                                     "Pulse.Extract.Main.fst"
-                                                                    (Prims.of_int (214))
+                                                                    (Prims.of_int (217))
                                                                     (Prims.of_int (22))
-                                                                    (Prims.of_int (214))
+                                                                    (Prims.of_int (217))
                                                                     (Prims.of_int (46)))))
                                                                     (FStar_Sealed.seal
                                                                     (Obj.magic
                                                                     (FStar_Range.mk_range
                                                                     "Pulse.Extract.Main.fst"
-                                                                    (Prims.of_int (212))
+                                                                    (Prims.of_int (215))
                                                                     (Prims.of_int (17))
-                                                                    (Prims.of_int (214))
+                                                                    (Prims.of_int (217))
                                                                     (Prims.of_int (47)))))
                                                                     (Obj.magic
                                                                     (Pulse_Syntax_Printer.st_term_to_string
@@ -1244,17 +1244,17 @@ let rec (extract :
                                                                     (Obj.magic
                                                                     (FStar_Range.mk_range
                                                                     "Pulse.Extract.Main.fst"
-                                                                    (Prims.of_int (212))
+                                                                    (Prims.of_int (215))
                                                                     (Prims.of_int (17))
-                                                                    (Prims.of_int (214))
+                                                                    (Prims.of_int (217))
                                                                     (Prims.of_int (47)))))
                                                                     (FStar_Sealed.seal
                                                                     (Obj.magic
                                                                     (FStar_Range.mk_range
                                                                     "Pulse.Extract.Main.fst"
-                                                                    (Prims.of_int (212))
+                                                                    (Prims.of_int (215))
                                                                     (Prims.of_int (17))
-                                                                    (Prims.of_int (214))
+                                                                    (Prims.of_int (217))
                                                                     (Prims.of_int (47)))))
                                                                     (Obj.magic
                                                                     (FStar_Tactics_Effect.tac_bind
@@ -1262,9 +1262,9 @@ let rec (extract :
                                                                     (Obj.magic
                                                                     (FStar_Range.mk_range
                                                                     "Pulse.Extract.Main.fst"
-                                                                    (Prims.of_int (213))
+                                                                    (Prims.of_int (216))
                                                                     (Prims.of_int (22))
-                                                                    (Prims.of_int (213))
+                                                                    (Prims.of_int (216))
                                                                     (Prims.of_int (46)))))
                                                                     (FStar_Sealed.seal
                                                                     (Obj.magic
@@ -1323,17 +1323,17 @@ let rec (extract :
                                                                     (Obj.magic
                                                                     (FStar_Range.mk_range
                                                                     "Pulse.Extract.Main.fst"
-                                                                    (Prims.of_int (218))
+                                                                    (Prims.of_int (221))
                                                                     (Prims.of_int (24))
-                                                                    (Prims.of_int (218))
+                                                                    (Prims.of_int (221))
                                                                     (Prims.of_int (38)))))
                                                                   (FStar_Sealed.seal
                                                                     (Obj.magic
                                                                     (FStar_Range.mk_range
                                                                     "Pulse.Extract.Main.fst"
-                                                                    (Prims.of_int (217))
+                                                                    (Prims.of_int (220))
                                                                     (Prims.of_int (13))
-                                                                    (Prims.of_int (225))
+                                                                    (Prims.of_int (228))
                                                                     (Prims.of_int (9)))))
                                                                   (Obj.magic
                                                                     (extract
@@ -1354,17 +1354,17 @@ let rec (extract :
                                                                     (Obj.magic
                                                                     (FStar_Range.mk_range
                                                                     "Pulse.Extract.Main.fst"
-                                                                    (Prims.of_int (219))
+                                                                    (Prims.of_int (222))
                                                                     (Prims.of_int (39))
-                                                                    (Prims.of_int (219))
+                                                                    (Prims.of_int (222))
                                                                     (Prims.of_int (58)))))
                                                                     (FStar_Sealed.seal
                                                                     (Obj.magic
                                                                     (FStar_Range.mk_range
                                                                     "Pulse.Extract.Main.fst"
-                                                                    (Prims.of_int (218))
+                                                                    (Prims.of_int (221))
                                                                     (Prims.of_int (41))
-                                                                    (Prims.of_int (224))
+                                                                    (Prims.of_int (227))
                                                                     (Prims.of_int (49)))))
                                                                     (Obj.magic
                                                                     (extend_env
@@ -1386,17 +1386,17 @@ let rec (extract :
                                                                     (Obj.magic
                                                                     (FStar_Range.mk_range
                                                                     "Pulse.Extract.Main.fst"
-                                                                    (Prims.of_int (220))
+                                                                    (Prims.of_int (223))
                                                                     (Prims.of_int (21))
-                                                                    (Prims.of_int (220))
+                                                                    (Prims.of_int (223))
                                                                     (Prims.of_int (49)))))
                                                                     (FStar_Sealed.seal
                                                                     (Obj.magic
                                                                     (FStar_Range.mk_range
                                                                     "Pulse.Extract.Main.fst"
-                                                                    (Prims.of_int (220))
+                                                                    (Prims.of_int (223))
                                                                     (Prims.of_int (52))
-                                                                    (Prims.of_int (224))
+                                                                    (Prims.of_int (227))
                                                                     (Prims.of_int (49)))))
                                                                     (FStar_Tactics_Effect.lift_div_tac
                                                                     (fun
@@ -1414,17 +1414,17 @@ let rec (extract :
                                                                     (Obj.magic
                                                                     (FStar_Range.mk_range
                                                                     "Pulse.Extract.Main.fst"
-                                                                    (Prims.of_int (221))
+                                                                    (Prims.of_int (224))
                                                                     (Prims.of_int (24))
-                                                                    (Prims.of_int (221))
+                                                                    (Prims.of_int (224))
                                                                     (Prims.of_int (38)))))
                                                                     (FStar_Sealed.seal
                                                                     (Obj.magic
                                                                     (FStar_Range.mk_range
                                                                     "Pulse.Extract.Main.fst"
-                                                                    (Prims.of_int (220))
+                                                                    (Prims.of_int (223))
                                                                     (Prims.of_int (52))
-                                                                    (Prims.of_int (224))
+                                                                    (Prims.of_int (227))
                                                                     (Prims.of_int (49)))))
                                                                     (Obj.magic
                                                                     (extract
@@ -1470,17 +1470,17 @@ let rec (extract :
                                                         (Obj.magic
                                                            (FStar_Range.mk_range
                                                               "Pulse.Extract.Main.fst"
-                                                              (Prims.of_int (229))
+                                                              (Prims.of_int (232))
                                                               (Prims.of_int (19))
-                                                              (Prims.of_int (229))
+                                                              (Prims.of_int (232))
                                                               (Prims.of_int (40)))))
                                                      (FStar_Sealed.seal
                                                         (Obj.magic
                                                            (FStar_Range.mk_range
                                                               "Pulse.Extract.Main.fst"
-                                                              (Prims.of_int (229))
+                                                              (Prims.of_int (232))
                                                               (Prims.of_int (43))
-                                                              (Prims.of_int (235))
+                                                              (Prims.of_int (238))
                                                               (Prims.of_int (47)))))
                                                      (Obj.magic
                                                         (term_as_mlexpr g
@@ -1493,17 +1493,17 @@ let rec (extract :
                                                                    (Obj.magic
                                                                     (FStar_Range.mk_range
                                                                     "Pulse.Extract.Main.fst"
-                                                                    (Prims.of_int (230))
+                                                                    (Prims.of_int (233))
                                                                     (Prims.of_int (37))
-                                                                    (Prims.of_int (230))
+                                                                    (Prims.of_int (233))
                                                                     (Prims.of_int (56)))))
                                                                 (FStar_Sealed.seal
                                                                    (Obj.magic
                                                                     (FStar_Range.mk_range
                                                                     "Pulse.Extract.Main.fst"
-                                                                    (Prims.of_int (229))
+                                                                    (Prims.of_int (232))
                                                                     (Prims.of_int (43))
-                                                                    (Prims.of_int (235))
+                                                                    (Prims.of_int (238))
                                                                     (Prims.of_int (47)))))
                                                                 (Obj.magic
                                                                    (extend_env
@@ -1525,17 +1525,17 @@ let rec (extract :
                                                                     (Obj.magic
                                                                     (FStar_Range.mk_range
                                                                     "Pulse.Extract.Main.fst"
-                                                                    (Prims.of_int (231))
+                                                                    (Prims.of_int (234))
                                                                     (Prims.of_int (19))
-                                                                    (Prims.of_int (231))
+                                                                    (Prims.of_int (234))
                                                                     (Prims.of_int (47)))))
                                                                     (FStar_Sealed.seal
                                                                     (Obj.magic
                                                                     (FStar_Range.mk_range
                                                                     "Pulse.Extract.Main.fst"
-                                                                    (Prims.of_int (231))
+                                                                    (Prims.of_int (234))
                                                                     (Prims.of_int (50))
-                                                                    (Prims.of_int (235))
+                                                                    (Prims.of_int (238))
                                                                     (Prims.of_int (47)))))
                                                                     (FStar_Tactics_Effect.lift_div_tac
                                                                     (fun
@@ -1553,17 +1553,17 @@ let rec (extract :
                                                                     (Obj.magic
                                                                     (FStar_Range.mk_range
                                                                     "Pulse.Extract.Main.fst"
-                                                                    (Prims.of_int (232))
+                                                                    (Prims.of_int (235))
                                                                     (Prims.of_int (22))
-                                                                    (Prims.of_int (232))
+                                                                    (Prims.of_int (235))
                                                                     (Prims.of_int (36)))))
                                                                     (FStar_Sealed.seal
                                                                     (Obj.magic
                                                                     (FStar_Range.mk_range
                                                                     "Pulse.Extract.Main.fst"
-                                                                    (Prims.of_int (231))
+                                                                    (Prims.of_int (234))
                                                                     (Prims.of_int (50))
-                                                                    (Prims.of_int (235))
+                                                                    (Prims.of_int (238))
                                                                     (Prims.of_int (47)))))
                                                                     (Obj.magic
                                                                     (extract
@@ -1608,17 +1608,17 @@ let rec (extract :
                                                         (Obj.magic
                                                            (FStar_Range.mk_range
                                                               "Pulse.Extract.Main.fst"
-                                                              (Prims.of_int (238))
+                                                              (Prims.of_int (241))
                                                               (Prims.of_int (16))
-                                                              (Prims.of_int (238))
+                                                              (Prims.of_int (241))
                                                               (Prims.of_int (34)))))
                                                      (FStar_Sealed.seal
                                                         (Obj.magic
                                                            (FStar_Range.mk_range
                                                               "Pulse.Extract.Main.fst"
-                                                              (Prims.of_int (238))
-                                                              (Prims.of_int (37))
                                                               (Prims.of_int (241))
+                                                              (Prims.of_int (37))
+                                                              (Prims.of_int (244))
                                                               (Prims.of_int (49)))))
                                                      (Obj.magic
                                                         (term_as_mlexpr g b))
@@ -1630,17 +1630,17 @@ let rec (extract :
                                                                    (Obj.magic
                                                                     (FStar_Range.mk_range
                                                                     "Pulse.Extract.Main.fst"
-                                                                    (Prims.of_int (239))
+                                                                    (Prims.of_int (242))
                                                                     (Prims.of_int (23))
-                                                                    (Prims.of_int (239))
+                                                                    (Prims.of_int (242))
                                                                     (Prims.of_int (38)))))
                                                                 (FStar_Sealed.seal
                                                                    (Obj.magic
                                                                     (FStar_Range.mk_range
                                                                     "Pulse.Extract.Main.fst"
-                                                                    (Prims.of_int (238))
-                                                                    (Prims.of_int (37))
                                                                     (Prims.of_int (241))
+                                                                    (Prims.of_int (37))
+                                                                    (Prims.of_int (244))
                                                                     (Prims.of_int (49)))))
                                                                 (Obj.magic
                                                                    (extract g
@@ -1661,17 +1661,17 @@ let rec (extract :
                                                                     (Obj.magic
                                                                     (FStar_Range.mk_range
                                                                     "Pulse.Extract.Main.fst"
-                                                                    (Prims.of_int (240))
+                                                                    (Prims.of_int (243))
                                                                     (Prims.of_int (23))
-                                                                    (Prims.of_int (240))
+                                                                    (Prims.of_int (243))
                                                                     (Prims.of_int (38)))))
                                                                     (FStar_Sealed.seal
                                                                     (Obj.magic
                                                                     (FStar_Range.mk_range
                                                                     "Pulse.Extract.Main.fst"
-                                                                    (Prims.of_int (239))
+                                                                    (Prims.of_int (242))
                                                                     (Prims.of_int (41))
-                                                                    (Prims.of_int (241))
+                                                                    (Prims.of_int (244))
                                                                     (Prims.of_int (49)))))
                                                                     (Obj.magic
                                                                     (extract
@@ -1706,17 +1706,17 @@ let rec (extract :
                                                         (Obj.magic
                                                            (FStar_Range.mk_range
                                                               "Pulse.Extract.Main.fst"
-                                                              (Prims.of_int (244))
+                                                              (Prims.of_int (247))
                                                               (Prims.of_int (17))
-                                                              (Prims.of_int (244))
+                                                              (Prims.of_int (247))
                                                               (Prims.of_int (36)))))
                                                      (FStar_Sealed.seal
                                                         (Obj.magic
                                                            (FStar_Range.mk_range
                                                               "Pulse.Extract.Main.fst"
-                                                              (Prims.of_int (244))
+                                                              (Prims.of_int (247))
                                                               (Prims.of_int (39))
-                                                              (Prims.of_int (252))
+                                                              (Prims.of_int (255))
                                                               (Prims.of_int (38)))))
                                                      (Obj.magic
                                                         (term_as_mlexpr g sc))
@@ -1728,17 +1728,17 @@ let rec (extract :
                                                                    (Obj.magic
                                                                     (FStar_Range.mk_range
                                                                     "Pulse.Extract.Main.fst"
-                                                                    (Prims.of_int (245))
+                                                                    (Prims.of_int (248))
                                                                     (Prims.of_int (40))
-                                                                    (Prims.of_int (249))
+                                                                    (Prims.of_int (252))
                                                                     (Prims.of_int (19)))))
                                                                 (FStar_Sealed.seal
                                                                    (Obj.magic
                                                                     (FStar_Range.mk_range
                                                                     "Pulse.Extract.Main.fst"
-                                                                    (Prims.of_int (250))
+                                                                    (Prims.of_int (253))
                                                                     (Prims.of_int (10))
-                                                                    (Prims.of_int (252))
+                                                                    (Prims.of_int (255))
                                                                     (Prims.of_int (38)))))
                                                                 (FStar_Tactics_Effect.lift_div_tac
                                                                    (fun
@@ -1755,17 +1755,17 @@ let rec (extract :
                                                                     (Obj.magic
                                                                     (FStar_Range.mk_range
                                                                     "Pulse.Extract.Main.fst"
-                                                                    (Prims.of_int (246))
+                                                                    (Prims.of_int (249))
                                                                     (Prims.of_int (27))
-                                                                    (Prims.of_int (246))
+                                                                    (Prims.of_int (249))
                                                                     (Prims.of_int (47)))))
                                                                     (FStar_Sealed.seal
                                                                     (Obj.magic
                                                                     (FStar_Range.mk_range
                                                                     "Pulse.Extract.Main.fst"
-                                                                    (Prims.of_int (245))
+                                                                    (Prims.of_int (248))
                                                                     (Prims.of_int (40))
-                                                                    (Prims.of_int (249))
+                                                                    (Prims.of_int (252))
                                                                     (Prims.of_int (19)))))
                                                                     (Obj.magic
                                                                     (extend_env_pat
@@ -1786,17 +1786,17 @@ let rec (extract :
                                                                     (Obj.magic
                                                                     (FStar_Range.mk_range
                                                                     "Pulse.Extract.Main.fst"
-                                                                    (Prims.of_int (247))
+                                                                    (Prims.of_int (250))
                                                                     (Prims.of_int (21))
-                                                                    (Prims.of_int (247))
+                                                                    (Prims.of_int (250))
                                                                     (Prims.of_int (64)))))
                                                                     (FStar_Sealed.seal
                                                                     (Obj.magic
                                                                     (FStar_Range.mk_range
                                                                     "Pulse.Extract.Main.fst"
-                                                                    (Prims.of_int (247))
+                                                                    (Prims.of_int (250))
                                                                     (Prims.of_int (67))
-                                                                    (Prims.of_int (249))
+                                                                    (Prims.of_int (252))
                                                                     (Prims.of_int (19)))))
                                                                     (FStar_Tactics_Effect.lift_div_tac
                                                                     (fun
@@ -1813,17 +1813,17 @@ let rec (extract :
                                                                     (Obj.magic
                                                                     (FStar_Range.mk_range
                                                                     "Pulse.Extract.Main.fst"
-                                                                    (Prims.of_int (248))
+                                                                    (Prims.of_int (251))
                                                                     (Prims.of_int (24))
-                                                                    (Prims.of_int (248))
+                                                                    (Prims.of_int (251))
                                                                     (Prims.of_int (38)))))
                                                                     (FStar_Sealed.seal
                                                                     (Obj.magic
                                                                     (FStar_Range.mk_range
                                                                     "Pulse.Extract.Main.fst"
-                                                                    (Prims.of_int (247))
+                                                                    (Prims.of_int (250))
                                                                     (Prims.of_int (67))
-                                                                    (Prims.of_int (249))
+                                                                    (Prims.of_int (252))
                                                                     (Prims.of_int (19)))))
                                                                     (Obj.magic
                                                                     (extract
@@ -1854,17 +1854,17 @@ let rec (extract :
                                                                     (Obj.magic
                                                                     (FStar_Range.mk_range
                                                                     "Pulse.Extract.Main.fst"
-                                                                    (Prims.of_int (251))
+                                                                    (Prims.of_int (254))
                                                                     (Prims.of_int (18))
-                                                                    (Prims.of_int (251))
+                                                                    (Prims.of_int (254))
                                                                     (Prims.of_int (42)))))
                                                                     (FStar_Sealed.seal
                                                                     (Obj.magic
                                                                     (FStar_Range.mk_range
                                                                     "Pulse.Extract.Main.fst"
-                                                                    (Prims.of_int (252))
+                                                                    (Prims.of_int (255))
                                                                     (Prims.of_int (8))
-                                                                    (Prims.of_int (252))
+                                                                    (Prims.of_int (255))
                                                                     (Prims.of_int (38)))))
                                                                     (Obj.magic
                                                                     (FStar_Tactics_Util.map
@@ -1897,17 +1897,17 @@ let rec (extract :
                                                         (Obj.magic
                                                            (FStar_Range.mk_range
                                                               "Pulse.Extract.Main.fst"
-                                                              (Prims.of_int (256))
+                                                              (Prims.of_int (259))
                                                               (Prims.of_int (27))
-                                                              (Prims.of_int (256))
+                                                              (Prims.of_int (259))
                                                               (Prims.of_int (46)))))
                                                      (FStar_Sealed.seal
                                                         (Obj.magic
                                                            (FStar_Range.mk_range
                                                               "Pulse.Extract.Main.fst"
-                                                              (Prims.of_int (255))
+                                                              (Prims.of_int (258))
                                                               (Prims.of_int (39))
-                                                              (Prims.of_int (261))
+                                                              (Prims.of_int (264))
                                                               (Prims.of_int (23)))))
                                                      (Obj.magic
                                                         (extract g condition))
@@ -1923,18 +1923,18 @@ let rec (extract :
                                                                     (Obj.magic
                                                                     (FStar_Range.mk_range
                                                                     "Pulse.Extract.Main.fst"
-                                                                    (Prims.of_int (257))
+                                                                    (Prims.of_int (260))
                                                                     (Prims.of_int (22))
-                                                                    (Prims.of_int (257))
+                                                                    (Prims.of_int (260))
                                                                     (Prims.of_int (36)))))
                                                                     (
                                                                     FStar_Sealed.seal
                                                                     (Obj.magic
                                                                     (FStar_Range.mk_range
                                                                     "Pulse.Extract.Main.fst"
-                                                                    (Prims.of_int (256))
+                                                                    (Prims.of_int (259))
                                                                     (Prims.of_int (49))
-                                                                    (Prims.of_int (261))
+                                                                    (Prims.of_int (264))
                                                                     (Prims.of_int (23)))))
                                                                     (
                                                                     Obj.magic
@@ -1992,17 +1992,17 @@ let rec (extract :
                                                         (Obj.magic
                                                            (FStar_Range.mk_range
                                                               "Pulse.Extract.Main.fst"
-                                                              (Prims.of_int (264))
+                                                              (Prims.of_int (267))
                                                               (Prims.of_int (23))
-                                                              (Prims.of_int (264))
+                                                              (Prims.of_int (267))
                                                               (Prims.of_int (38)))))
                                                      (FStar_Sealed.seal
                                                         (Obj.magic
                                                            (FStar_Range.mk_range
                                                               "Pulse.Extract.Main.fst"
-                                                              (Prims.of_int (263))
+                                                              (Prims.of_int (266))
                                                               (Prims.of_int (34))
-                                                              (Prims.of_int (269))
+                                                              (Prims.of_int (272))
                                                               (Prims.of_int (23)))))
                                                      (Obj.magic
                                                         (extract g body1))
@@ -2018,18 +2018,18 @@ let rec (extract :
                                                                     (Obj.magic
                                                                     (FStar_Range.mk_range
                                                                     "Pulse.Extract.Main.fst"
-                                                                    (Prims.of_int (265))
+                                                                    (Prims.of_int (268))
                                                                     (Prims.of_int (23))
-                                                                    (Prims.of_int (265))
+                                                                    (Prims.of_int (268))
                                                                     (Prims.of_int (38)))))
                                                                     (
                                                                     FStar_Sealed.seal
                                                                     (Obj.magic
                                                                     (FStar_Range.mk_range
                                                                     "Pulse.Extract.Main.fst"
-                                                                    (Prims.of_int (264))
+                                                                    (Prims.of_int (267))
                                                                     (Prims.of_int (41))
-                                                                    (Prims.of_int (269))
+                                                                    (Prims.of_int (272))
                                                                     (Prims.of_int (23)))))
                                                                     (
                                                                     Obj.magic
@@ -2082,17 +2082,17 @@ let rec (extract :
                                                         (Obj.magic
                                                            (FStar_Range.mk_range
                                                               "Pulse.Extract.Main.fst"
-                                                              (Prims.of_int (272))
+                                                              (Prims.of_int (275))
                                                               (Prims.of_int (26))
-                                                              (Prims.of_int (272))
+                                                              (Prims.of_int (275))
                                                               (Prims.of_int (54)))))
                                                      (FStar_Sealed.seal
                                                         (Obj.magic
                                                            (FStar_Range.mk_range
                                                               "Pulse.Extract.Main.fst"
-                                                              (Prims.of_int (272))
+                                                              (Prims.of_int (275))
                                                               (Prims.of_int (57))
-                                                              (Prims.of_int (279))
+                                                              (Prims.of_int (282))
                                                               (Prims.of_int (47)))))
                                                      (Obj.magic
                                                         (term_as_mlexpr g
@@ -2105,17 +2105,17 @@ let rec (extract :
                                                                    (Obj.magic
                                                                     (FStar_Range.mk_range
                                                                     "Pulse.Extract.Main.fst"
-                                                                    (Prims.of_int (273))
+                                                                    (Prims.of_int (276))
                                                                     (Prims.of_int (37))
-                                                                    (Prims.of_int (273))
+                                                                    (Prims.of_int (276))
                                                                     (Prims.of_int (94)))))
                                                                 (FStar_Sealed.seal
                                                                    (Obj.magic
                                                                     (FStar_Range.mk_range
                                                                     "Pulse.Extract.Main.fst"
-                                                                    (Prims.of_int (272))
+                                                                    (Prims.of_int (275))
                                                                     (Prims.of_int (57))
-                                                                    (Prims.of_int (279))
+                                                                    (Prims.of_int (282))
                                                                     (Prims.of_int (47)))))
                                                                 (Obj.magic
                                                                    (extend_env
@@ -2145,17 +2145,17 @@ let rec (extract :
                                                                     (Obj.magic
                                                                     (FStar_Range.mk_range
                                                                     "Pulse.Extract.Main.fst"
-                                                                    (Prims.of_int (274))
+                                                                    (Prims.of_int (277))
                                                                     (Prims.of_int (19))
-                                                                    (Prims.of_int (274))
+                                                                    (Prims.of_int (277))
                                                                     (Prims.of_int (47)))))
                                                                     (FStar_Sealed.seal
                                                                     (Obj.magic
                                                                     (FStar_Range.mk_range
                                                                     "Pulse.Extract.Main.fst"
-                                                                    (Prims.of_int (274))
+                                                                    (Prims.of_int (277))
                                                                     (Prims.of_int (50))
-                                                                    (Prims.of_int (279))
+                                                                    (Prims.of_int (282))
                                                                     (Prims.of_int (47)))))
                                                                     (FStar_Tactics_Effect.lift_div_tac
                                                                     (fun
@@ -2173,17 +2173,17 @@ let rec (extract :
                                                                     (Obj.magic
                                                                     (FStar_Range.mk_range
                                                                     "Pulse.Extract.Main.fst"
-                                                                    (Prims.of_int (275))
+                                                                    (Prims.of_int (278))
                                                                     (Prims.of_int (22))
-                                                                    (Prims.of_int (275))
+                                                                    (Prims.of_int (278))
                                                                     (Prims.of_int (36)))))
                                                                     (FStar_Sealed.seal
                                                                     (Obj.magic
                                                                     (FStar_Range.mk_range
                                                                     "Pulse.Extract.Main.fst"
-                                                                    (Prims.of_int (274))
+                                                                    (Prims.of_int (277))
                                                                     (Prims.of_int (50))
-                                                                    (Prims.of_int (279))
+                                                                    (Prims.of_int (282))
                                                                     (Prims.of_int (47)))))
                                                                     (Obj.magic
                                                                     (extract
@@ -2238,17 +2238,17 @@ let rec (extract :
                                                         (Obj.magic
                                                            (FStar_Range.mk_range
                                                               "Pulse.Extract.Main.fst"
-                                                              (Prims.of_int (282))
+                                                              (Prims.of_int (285))
                                                               (Prims.of_int (30))
-                                                              (Prims.of_int (282))
+                                                              (Prims.of_int (285))
                                                               (Prims.of_int (149)))))
                                                      (FStar_Sealed.seal
                                                         (Obj.magic
                                                            (FStar_Range.mk_range
                                                               "Pulse.Extract.Main.fst"
-                                                              (Prims.of_int (282))
+                                                              (Prims.of_int (285))
                                                               (Prims.of_int (22))
-                                                              (Prims.of_int (282))
+                                                              (Prims.of_int (285))
                                                               (Prims.of_int (149)))))
                                                      (Obj.magic
                                                         (FStar_Tactics_Effect.tac_bind
@@ -2256,17 +2256,17 @@ let rec (extract :
                                                               (Obj.magic
                                                                  (FStar_Range.mk_range
                                                                     "Pulse.Extract.Main.fst"
-                                                                    (Prims.of_int (282))
+                                                                    (Prims.of_int (285))
                                                                     (Prims.of_int (50))
-                                                                    (Prims.of_int (282))
+                                                                    (Prims.of_int (285))
                                                                     (Prims.of_int (148)))))
                                                            (FStar_Sealed.seal
                                                               (Obj.magic
                                                                  (FStar_Range.mk_range
                                                                     "Pulse.Extract.Main.fst"
-                                                                    (Prims.of_int (282))
+                                                                    (Prims.of_int (285))
                                                                     (Prims.of_int (30))
-                                                                    (Prims.of_int (282))
+                                                                    (Prims.of_int (285))
                                                                     (Prims.of_int (149)))))
                                                            (Obj.magic
                                                               (FStar_Tactics_Effect.tac_bind
@@ -2275,9 +2275,9 @@ let rec (extract :
                                                                     Obj.magic
                                                                     (FStar_Range.mk_range
                                                                     "Pulse.Extract.Main.fst"
-                                                                    (Prims.of_int (282))
+                                                                    (Prims.of_int (285))
                                                                     (Prims.of_int (105))
-                                                                    (Prims.of_int (282))
+                                                                    (Prims.of_int (285))
                                                                     (Prims.of_int (147)))))
                                                                  (FStar_Sealed.seal
                                                                     (
@@ -2314,157 +2314,363 @@ let rec (extract :
                         uu___))) uu___)
 let (extract_pulse :
   Pulse_Extract_CompilerLib.uenv ->
-    Pulse_Syntax_Base.st_term ->
-      (((Pulse_Extract_CompilerLib.mlexpr * Pulse_Extract_CompilerLib.e_tag *
-          Pulse_Extract_CompilerLib.mlty),
-         Prims.string) FStar_Pervasives.either,
-        unit) FStar_Tactics_Effect.tac_repr)
+    FStar_Reflection_Types.sigelt ->
+      Pulse_Syntax_Base.st_term ->
+        ((Pulse_Extract_CompilerLib.mlmodule, Prims.string)
+           FStar_Pervasives.either,
+          unit) FStar_Tactics_Effect.tac_repr)
   =
   fun g ->
-    fun p ->
-      FStar_Tactics_Effect.tac_bind
-        (FStar_Sealed.seal
-           (Obj.magic
-              (FStar_Range.mk_range "Pulse.Extract.Main.fst"
-                 (Prims.of_int (290)) (Prims.of_int (4)) (Prims.of_int (290))
-                 (Prims.of_int (75)))))
-        (FStar_Sealed.seal
-           (Obj.magic
-              (FStar_Range.mk_range "Pulse.Extract.Main.fst"
-                 (Prims.of_int (291)) (Prims.of_int (4)) (Prims.of_int (299))
-                 (Prims.of_int (77)))))
-        (Obj.magic
-           (FStar_Tactics_Effect.tac_bind
-              (FStar_Sealed.seal
-                 (Obj.magic
-                    (FStar_Range.mk_range "Pulse.Extract.Main.fst"
-                       (Prims.of_int (290)) (Prims.of_int (11))
-                       (Prims.of_int (290)) (Prims.of_int (75)))))
-              (FStar_Sealed.seal
-                 (Obj.magic
-                    (FStar_Range.mk_range "Pulse.Extract.Main.fst"
-                       (Prims.of_int (290)) (Prims.of_int (4))
-                       (Prims.of_int (290)) (Prims.of_int (75)))))
-              (Obj.magic
-                 (FStar_Tactics_Effect.tac_bind
-                    (FStar_Sealed.seal
-                       (Obj.magic
-                          (FStar_Range.mk_range "Pulse.Extract.Main.fst"
-                             (Prims.of_int (290)) (Prims.of_int (53))
-                             (Prims.of_int (290)) (Prims.of_int (74)))))
-                    (FStar_Sealed.seal
-                       (Obj.magic
-                          (FStar_Range.mk_range "prims.fst"
-                             (Prims.of_int (590)) (Prims.of_int (19))
-                             (Prims.of_int (590)) (Prims.of_int (31)))))
-                    (Obj.magic (Pulse_Syntax_Printer.st_term_to_string p))
-                    (fun uu___ ->
-                       FStar_Tactics_Effect.lift_div_tac
-                         (fun uu___1 ->
-                            Prims.strcat "About to extract:\n"
-                              (Prims.strcat uu___ "\n")))))
-              (fun uu___ ->
-                 (fun uu___ ->
-                    Obj.magic (FStar_Tactics_V2_Builtins.dump uu___)) uu___)))
-        (fun uu___ ->
-           (fun uu___ ->
-              Obj.magic
-                (FStar_Tactics_V2_Derived.try_with
-                   (fun uu___1 ->
-                      match () with
-                      | () ->
-                          FStar_Tactics_Effect.tac_bind
-                            (FStar_Sealed.seal
-                               (Obj.magic
-                                  (FStar_Range.mk_range
-                                     "Pulse.Extract.Main.fst"
-                                     (Prims.of_int (292)) (Prims.of_int (20))
-                                     (Prims.of_int (292)) (Prims.of_int (74)))))
-                            (FStar_Sealed.seal
-                               (Obj.magic
-                                  (FStar_Range.mk_range
-                                     "Pulse.Extract.Main.fst"
-                                     (Prims.of_int (291)) (Prims.of_int (7))
-                                     (Prims.of_int (294)) (Prims.of_int (29)))))
-                            (Obj.magic
-                               (extract
-                                  {
-                                    uenv_inner = g;
-                                    coreenv =
-                                      (Pulse_Extract_CompilerLib.initial_core_env
-                                         g)
-                                  } p))
-                            (fun uu___2 ->
-                               (fun uu___2 ->
-                                  match uu___2 with
-                                  | (tm, tag) ->
-                                      Obj.magic
-                                        (FStar_Tactics_Effect.tac_bind
-                                           (FStar_Sealed.seal
-                                              (Obj.magic
-                                                 (FStar_Range.mk_range
-                                                    "Pulse.Extract.Main.fst"
-                                                    (Prims.of_int (293))
-                                                    (Prims.of_int (6))
-                                                    (Prims.of_int (293))
-                                                    (Prims.of_int (74)))))
-                                           (FStar_Sealed.seal
-                                              (Obj.magic
-                                                 (FStar_Range.mk_range
-                                                    "Pulse.Extract.Main.fst"
-                                                    (Prims.of_int (294))
-                                                    (Prims.of_int (6))
-                                                    (Prims.of_int (294))
-                                                    (Prims.of_int (29)))))
-                                           (Obj.magic
-                                              (FStar_Tactics_Effect.tac_bind
-                                                 (FStar_Sealed.seal
-                                                    (Obj.magic
-                                                       (FStar_Range.mk_range
-                                                          "Pulse.Extract.Main.fst"
-                                                          (Prims.of_int (293))
-                                                          (Prims.of_int (13))
-                                                          (Prims.of_int (293))
-                                                          (Prims.of_int (74)))))
-                                                 (FStar_Sealed.seal
-                                                    (Obj.magic
-                                                       (FStar_Range.mk_range
-                                                          "Pulse.Extract.Main.fst"
-                                                          (Prims.of_int (293))
-                                                          (Prims.of_int (6))
-                                                          (Prims.of_int (293))
-                                                          (Prims.of_int (74)))))
-                                                 (FStar_Tactics_Effect.lift_div_tac
-                                                    (fun uu___3 ->
-                                                       Prims.strcat
-                                                         "Extracted term: "
-                                                         (Prims.strcat
-                                                            (Pulse_Extract_CompilerLib.mlexpr_to_string
-                                                               tm) "\n")))
-                                                 (fun uu___3 ->
-                                                    (fun uu___3 ->
-                                                       Obj.magic
-                                                         (FStar_Tactics_V2_Builtins.dump
-                                                            uu___3)) uu___3)))
-                                           (fun uu___3 ->
-                                              FStar_Tactics_Effect.lift_div_tac
-                                                (fun uu___4 ->
-                                                   FStar_Pervasives.Inl
-                                                     (tm, tag,
-                                                       Pulse_Extract_CompilerLib.mlty_top)))))
-                                 uu___2))
-                   (fun uu___1 ->
-                      (fun uu___1 ->
-                         Obj.magic
-                           (FStar_Tactics_Effect.lift_div_tac
+    fun selt ->
+      fun p ->
+        FStar_Tactics_Effect.tac_bind
+          (FStar_Sealed.seal
+             (Obj.magic
+                (FStar_Range.mk_range "Pulse.Extract.Main.fst"
+                   (Prims.of_int (293)) (Prims.of_int (2))
+                   (Prims.of_int (293)) (Prims.of_int (73)))))
+          (FStar_Sealed.seal
+             (Obj.magic
+                (FStar_Range.mk_range "Pulse.Extract.Main.fst"
+                   (Prims.of_int (294)) (Prims.of_int (2))
+                   (Prims.of_int (315)) (Prims.of_int (75)))))
+          (Obj.magic
+             (FStar_Tactics_Effect.tac_bind
+                (FStar_Sealed.seal
+                   (Obj.magic
+                      (FStar_Range.mk_range "Pulse.Extract.Main.fst"
+                         (Prims.of_int (293)) (Prims.of_int (9))
+                         (Prims.of_int (293)) (Prims.of_int (73)))))
+                (FStar_Sealed.seal
+                   (Obj.magic
+                      (FStar_Range.mk_range "Pulse.Extract.Main.fst"
+                         (Prims.of_int (293)) (Prims.of_int (2))
+                         (Prims.of_int (293)) (Prims.of_int (73)))))
+                (Obj.magic
+                   (FStar_Tactics_Effect.tac_bind
+                      (FStar_Sealed.seal
+                         (Obj.magic
+                            (FStar_Range.mk_range "Pulse.Extract.Main.fst"
+                               (Prims.of_int (293)) (Prims.of_int (51))
+                               (Prims.of_int (293)) (Prims.of_int (72)))))
+                      (FStar_Sealed.seal
+                         (Obj.magic
+                            (FStar_Range.mk_range "prims.fst"
+                               (Prims.of_int (590)) (Prims.of_int (19))
+                               (Prims.of_int (590)) (Prims.of_int (31)))))
+                      (Obj.magic (Pulse_Syntax_Printer.st_term_to_string p))
+                      (fun uu___ ->
+                         FStar_Tactics_Effect.lift_div_tac
+                           (fun uu___1 ->
+                              Prims.strcat "About to extract:\n"
+                                (Prims.strcat uu___ "\n")))))
+                (fun uu___ ->
+                   (fun uu___ ->
+                      Obj.magic (FStar_Tactics_V2_Builtins.dump uu___)) uu___)))
+          (fun uu___ ->
+             (fun uu___ ->
+                Obj.magic
+                  (FStar_Tactics_V2_Derived.try_with
+                     (fun uu___1 ->
+                        match () with
+                        | () ->
+                            FStar_Tactics_Effect.tac_bind
+                              (FStar_Sealed.seal
+                                 (Obj.magic
+                                    (FStar_Range.mk_range
+                                       "Pulse.Extract.Main.fst"
+                                       (Prims.of_int (295))
+                                       (Prims.of_int (22))
+                                       (Prims.of_int (295))
+                                       (Prims.of_int (43)))))
+                              (FStar_Sealed.seal
+                                 (Obj.magic
+                                    (FStar_Range.mk_range
+                                       "Pulse.Extract.Main.fst"
+                                       (Prims.of_int (296))
+                                       (Prims.of_int (4))
+                                       (Prims.of_int (310))
+                                       (Prims.of_int (59)))))
+                              (FStar_Tactics_Effect.lift_div_tac
+                                 (fun uu___2 ->
+                                    FStar_Reflection_V2_Builtins.inspect_sigelt
+                                      selt))
                               (fun uu___2 ->
-                                 match uu___1 with
-                                 | Extraction_failure msg ->
-                                     FStar_Pervasives.Inr msg
-                                 | e ->
-                                     FStar_Pervasives.Inr
-                                       (Prims.strcat
-                                          "Unexpected extraction error: "
-                                          (Prims.strcat
-                                             (Pulse_RuntimeUtils.print_exn e)
-                                             ""))))) uu___1))) uu___)
+                                 (fun sigelt_view ->
+                                    match sigelt_view with
+                                    | FStar_Reflection_V2_Data.Sg_Let
+                                        (is_rec, lbs) ->
+                                        Obj.magic
+                                          (Obj.repr
+                                             (if
+                                                is_rec ||
+                                                  ((FStar_List_Tot_Base.length
+                                                      lbs)
+                                                     <> Prims.int_one)
+                                              then
+                                                Obj.repr
+                                                  (FStar_Tactics_Effect.raise
+                                                     (Extraction_failure
+                                                        "Extraction of recursive lets is not yet supported"))
+                                              else
+                                                Obj.repr
+                                                  (FStar_Tactics_Effect.tac_bind
+                                                     (FStar_Sealed.seal
+                                                        (Obj.magic
+                                                           (FStar_Range.mk_range
+                                                              "Pulse.Extract.Main.fst"
+                                                              (Prims.of_int (301))
+                                                              (Prims.of_int (30))
+                                                              (Prims.of_int (301))
+                                                              (Prims.of_int (60)))))
+                                                     (FStar_Sealed.seal
+                                                        (Obj.magic
+                                                           (FStar_Range.mk_range
+                                                              "Pulse.Extract.Main.fst"
+                                                              (Prims.of_int (300))
+                                                              (Prims.of_int (10))
+                                                              (Prims.of_int (309))
+                                                              (Prims.of_int (34)))))
+                                                     (FStar_Tactics_Effect.lift_div_tac
+                                                        (fun uu___3 ->
+                                                           FStar_Reflection_V2_Builtins.inspect_lb
+                                                             (FStar_List_Tot_Base.hd
+                                                                lbs)))
+                                                     (fun uu___3 ->
+                                                        (fun uu___3 ->
+                                                           match uu___3 with
+                                                           | {
+                                                               FStar_Reflection_V2_Data.lb_fv
+                                                                 = lb_fv;
+                                                               FStar_Reflection_V2_Data.lb_us
+                                                                 = uu___4;
+                                                               FStar_Reflection_V2_Data.lb_typ
+                                                                 = lb_typ;
+                                                               FStar_Reflection_V2_Data.lb_def
+                                                                 = uu___5;_}
+                                                               ->
+                                                               Obj.magic
+                                                                 (FStar_Tactics_Effect.tac_bind
+                                                                    (
+                                                                    FStar_Sealed.seal
+                                                                    (Obj.magic
+                                                                    (FStar_Range.mk_range
+                                                                    "Pulse.Extract.Main.fst"
+                                                                    (Prims.of_int (302))
+                                                                    (Prims.of_int (19))
+                                                                    (Prims.of_int (302))
+                                                                    (Prims.of_int (44)))))
+                                                                    (
+                                                                    FStar_Sealed.seal
+                                                                    (Obj.magic
+                                                                    (FStar_Range.mk_range
+                                                                    "Pulse.Extract.Main.fst"
+                                                                    (Prims.of_int (302))
+                                                                    (Prims.of_int (47))
+                                                                    (Prims.of_int (309))
+                                                                    (Prims.of_int (34)))))
+                                                                    (
+                                                                    FStar_Tactics_Effect.lift_div_tac
+                                                                    (fun
+                                                                    uu___6 ->
+                                                                    Pulse_Extract_CompilerLib.term_as_mlty
+                                                                    g lb_typ))
+                                                                    (
+                                                                    fun
+                                                                    uu___6 ->
+                                                                    (fun mlty
+                                                                    ->
+                                                                    Obj.magic
+                                                                    (FStar_Tactics_Effect.tac_bind
+                                                                    (FStar_Sealed.seal
+                                                                    (Obj.magic
+                                                                    (FStar_Range.mk_range
+                                                                    "Pulse.Extract.Main.fst"
+                                                                    (Prims.of_int (303))
+                                                                    (Prims.of_int (22))
+                                                                    (Prims.of_int (303))
+                                                                    (Prims.of_int (76)))))
+                                                                    (FStar_Sealed.seal
+                                                                    (Obj.magic
+                                                                    (FStar_Range.mk_range
+                                                                    "Pulse.Extract.Main.fst"
+                                                                    (Prims.of_int (302))
+                                                                    (Prims.of_int (47))
+                                                                    (Prims.of_int (309))
+                                                                    (Prims.of_int (34)))))
+                                                                    (Obj.magic
+                                                                    (extract
+                                                                    {
+                                                                    uenv_inner
+                                                                    = g;
+                                                                    coreenv =
+                                                                    (Pulse_Extract_CompilerLib.initial_core_env
+                                                                    g)
+                                                                    } p))
+                                                                    (fun
+                                                                    uu___6 ->
+                                                                    (fun
+                                                                    uu___6 ->
+                                                                    match uu___6
+                                                                    with
+                                                                    | 
+                                                                    (tm, tag)
+                                                                    ->
+                                                                    Obj.magic
+                                                                    (FStar_Tactics_Effect.tac_bind
+                                                                    (FStar_Sealed.seal
+                                                                    (Obj.magic
+                                                                    (FStar_Range.mk_range
+                                                                    "Pulse.Extract.Main.fst"
+                                                                    (Prims.of_int (304))
+                                                                    (Prims.of_int (8))
+                                                                    (Prims.of_int (304))
+                                                                    (Prims.of_int (76)))))
+                                                                    (FStar_Sealed.seal
+                                                                    (Obj.magic
+                                                                    (FStar_Range.mk_range
+                                                                    "Pulse.Extract.Main.fst"
+                                                                    (Prims.of_int (304))
+                                                                    (Prims.of_int (77))
+                                                                    (Prims.of_int (309))
+                                                                    (Prims.of_int (34)))))
+                                                                    (Obj.magic
+                                                                    (FStar_Tactics_Effect.tac_bind
+                                                                    (FStar_Sealed.seal
+                                                                    (Obj.magic
+                                                                    (FStar_Range.mk_range
+                                                                    "Pulse.Extract.Main.fst"
+                                                                    (Prims.of_int (304))
+                                                                    (Prims.of_int (15))
+                                                                    (Prims.of_int (304))
+                                                                    (Prims.of_int (76)))))
+                                                                    (FStar_Sealed.seal
+                                                                    (Obj.magic
+                                                                    (FStar_Range.mk_range
+                                                                    "Pulse.Extract.Main.fst"
+                                                                    (Prims.of_int (304))
+                                                                    (Prims.of_int (8))
+                                                                    (Prims.of_int (304))
+                                                                    (Prims.of_int (76)))))
+                                                                    (FStar_Tactics_Effect.lift_div_tac
+                                                                    (fun
+                                                                    uu___7 ->
+                                                                    Prims.strcat
+                                                                    "Extracted term: "
+                                                                    (Prims.strcat
+                                                                    (Pulse_Extract_CompilerLib.mlexpr_to_string
+                                                                    tm) "\n")))
+                                                                    (fun
+                                                                    uu___7 ->
+                                                                    (fun
+                                                                    uu___7 ->
+                                                                    Obj.magic
+                                                                    (FStar_Tactics_V2_Builtins.dump
+                                                                    uu___7))
+                                                                    uu___7)))
+                                                                    (fun
+                                                                    uu___7 ->
+                                                                    (fun
+                                                                    uu___7 ->
+                                                                    Obj.magic
+                                                                    (FStar_Tactics_Effect.tac_bind
+                                                                    (FStar_Sealed.seal
+                                                                    (Obj.magic
+                                                                    (FStar_Range.mk_range
+                                                                    "Pulse.Extract.Main.fst"
+                                                                    (Prims.of_int (305))
+                                                                    (Prims.of_int (22))
+                                                                    (Prims.of_int (305))
+                                                                    (Prims.of_int (40)))))
+                                                                    (FStar_Sealed.seal
+                                                                    (Obj.magic
+                                                                    (FStar_Range.mk_range
+                                                                    "Pulse.Extract.Main.fst"
+                                                                    (Prims.of_int (306))
+                                                                    (Prims.of_int (8))
+                                                                    (Prims.of_int (309))
+                                                                    (Prims.of_int (34)))))
+                                                                    (FStar_Tactics_Effect.lift_div_tac
+                                                                    (fun
+                                                                    uu___8 ->
+                                                                    FStar_Reflection_V2_Builtins.inspect_fv
+                                                                    lb_fv))
+                                                                    (fun
+                                                                    uu___8 ->
+                                                                    (fun
+                                                                    fv_name
+                                                                    ->
+                                                                    Obj.magic
+                                                                    (FStar_Tactics_Effect.tac_bind
+                                                                    (FStar_Sealed.seal
+                                                                    (Obj.magic
+                                                                    (FStar_Range.mk_range
+                                                                    "Pulse.Extract.Main.fst"
+                                                                    (Prims.of_int (306))
+                                                                    (Prims.of_int (8))
+                                                                    (Prims.of_int (307))
+                                                                    (Prims.of_int (65)))))
+                                                                    (FStar_Sealed.seal
+                                                                    (Obj.magic
+                                                                    (FStar_Range.mk_range
+                                                                    "Pulse.Extract.Main.fst"
+                                                                    (Prims.of_int (309))
+                                                                    (Prims.of_int (8))
+                                                                    (Prims.of_int (309))
+                                                                    (Prims.of_int (34)))))
+                                                                    (if
+                                                                    (FStar_List_Tot_Base.length
+                                                                    fv_name)
+                                                                    =
+                                                                    Prims.int_zero
+                                                                    then
+                                                                    FStar_Tactics_Effect.raise
+                                                                    (Extraction_failure
+                                                                    "Unexpected empty name")
+                                                                    else
+                                                                    FStar_Tactics_Effect.lift_div_tac
+                                                                    (fun
+                                                                    uu___9 ->
+                                                                    ()))
+                                                                    (fun
+                                                                    uu___8 ->
+                                                                    FStar_Tactics_Effect.lift_div_tac
+                                                                    (fun
+                                                                    uu___9 ->
+                                                                    FStar_Pervasives.Inl
+                                                                    [
+                                                                    Pulse_Extract_CompilerLib.mlm_let
+                                                                    false
+                                                                    [
+                                                                    Pulse_Extract_CompilerLib.mk_mllb
+                                                                    (FStar_List_Tot_Base.last
+                                                                    fv_name)
+                                                                    ([],
+                                                                    mlty) tm]]))))
+                                                                    uu___8)))
+                                                                    uu___7)))
+                                                                    uu___6)))
+                                                                    uu___6)))
+                                                          uu___3))))
+                                    | uu___2 ->
+                                        Obj.magic
+                                          (Obj.repr
+                                             (FStar_Tactics_Effect.raise
+                                                (Extraction_failure
+                                                   "Unexpected sigelt"))))
+                                   uu___2))
+                     (fun uu___1 ->
+                        (fun uu___1 ->
+                           Obj.magic
+                             (FStar_Tactics_Effect.lift_div_tac
+                                (fun uu___2 ->
+                                   match uu___1 with
+                                   | Extraction_failure msg ->
+                                       FStar_Pervasives.Inr msg
+                                   | e ->
+                                       FStar_Pervasives.Inr
+                                         (Prims.strcat
+                                            "Unexpected extraction error: "
+                                            (Prims.strcat
+                                               (Pulse_RuntimeUtils.print_exn
+                                                  e) ""))))) uu___1))) uu___)
